Non-contextual polytope
------------------------------
constraints:
\langle l_1 \rangle - \langle l_2 \rangle - \langle l_1 l_2 \rangle &\geq -1\\
\langle l_1 \rangle + \langle l_2 \rangle + \langle l_1 l_2 \rangle &\geq -1\\
\langle l_1 \rangle - \langle l'_2 \rangle - \langle l_1 l'_2 \rangle &\geq -1\\
\langle l_1 \rangle + \langle l'_2 \rangle + \langle l_1 l'_2 \rangle &\geq -1\\
-\langle l_1 \rangle + \langle l_2 \rangle - \langle l_1 l_2 \rangle &\geq -1\\
-\langle l_1 \rangle - \langle l_2 \rangle + \langle l_1 l_2 \rangle &\geq -1\\
-\langle l_1 \rangle + \langle l'_2 \rangle - \langle l_1 l'_2 \rangle &\geq -1\\
-\langle l_1 \rangle - \langle l'_2 \rangle + \langle l_1 l'_2 \rangle &\geq -1\\
\langle l_2 \rangle + \langle l'_1 \rangle + \langle l'_1 l_2 \rangle &\geq -1\\
\langle l_2 \rangle - \langle l'_1 \rangle - \langle l'_1 l_2 \rangle &\geq -1\\
-\langle l_2 \rangle + \langle l'_1 \rangle - \langle l'_1 l_2 \rangle &\geq -1\\
-\langle l_2 \rangle - \langle l'_1 \rangle + \langle l'_1 l_2 \rangle &\geq -1\\
\langle l'_1 \rangle - \langle l'_2 \rangle - \langle l'_1 l'_2 \rangle &\geq -1\\
\langle l'_1 \rangle + \langle l'_2 \rangle + \langle l'_1 l'_2 \rangle &\geq -1\\
-\langle l'_1 \rangle + \langle l'_2 \rangle - \langle l'_1 l'_2 \rangle &\geq -1\\
-\langle l'_1 \rangle - \langle l'_2 \rangle + \langle l'_1 l'_2 \rangle &\geq -1\\
\langle l_1 l_2 \rangle - \langle l'_1 l_2 \rangle + \langle l'_1 l'_2 \rangle + \langle l_1 l'_2 \rangle &\geq -2\\
\langle l_1 l_2 \rangle + \langle l'_1 l_2 \rangle - \langle l'_1 l'_2 \rangle + \langle l_1 l'_2 \rangle &\geq -2\\
\langle l_1 l_2 \rangle + \langle l'_1 l_2 \rangle + \langle l'_1 l'_2 \rangle - \langle l_1 l'_2 \rangle &\geq -2\\
\langle l_1 l_2 \rangle - \langle l'_1 l_2 \rangle - \langle l'_1 l'_2 \rangle - \langle l_1 l'_2 \rangle &\geq -2\\
-\langle l_1 l_2 \rangle + \langle l'_1 l_2 \rangle - \langle l'_1 l'_2 \rangle - \langle l_1 l'_2 \rangle &\geq -2\\
-\langle l_1 l_2 \rangle - \langle l'_1 l_2 \rangle + \langle l'_1 l'_2 \rangle - \langle l_1 l'_2 \rangle &\geq -2\\
-\langle l_1 l_2 \rangle + \langle l'_1 l_2 \rangle + \langle l'_1 l'_2 \rangle + \langle l_1 l'_2 \rangle &\geq -2\\
-\langle l_1 l_2 \rangle - \langle l'_1 l_2 \rangle - \langle l'_1 l'_2 \rangle + \langle l_1 l'_2 \rangle &\geq -2

No-disturbance polytope
------------------------------
constraints:

\langle l_1 \rangle + \langle l'_2 \rangle + \langle l_1 l'_2 \rangle &\geq -1\\
\langle l_1 \rangle + \langle l_2 \rangle + \langle l_1 l_2 \rangle &\geq -1\\
\langle l_1 \rangle - \langle l'_2 \rangle - \langle l_1 l'_2 \rangle &\geq -1\\
\langle l_1 \rangle - \langle l_2 \rangle - \langle l_1 l_2 \rangle &\geq -1\\
-\langle l_1 \rangle + \langle l_2 \rangle - \langle l_1 l_2 \rangle &\geq -1\\
-\langle l_1 \rangle - \langle l_2 \rangle + \langle l_1 l_2 \rangle &\geq -1\\
-\langle l_1 \rangle - \langle l'_2 \rangle + \langle l_1 l'_2 \rangle &\geq -1\\
-\langle l_1 \rangle + \langle l'_2 \rangle - \langle l_1 l'_2 \rangle &\geq -1\\
\langle l_2 \rangle + \langle l'_1 \rangle + \langle l'_1 l_2 \rangle &\geq -1\\
-\langle l_2 \rangle + \langle l'_1 \rangle - \langle l'_1 l_2 \rangle &\geq -1\\
-\langle l_2 \rangle - \langle l'_1 \rangle + \langle l'_1 l_2 \rangle &\geq -1\\
\langle l_2 \rangle - \langle l'_1 \rangle - \langle l'_1 l_2 \rangle &\geq -1\\
\langle l'_1 \rangle - \langle l'_2 \rangle - \langle l'_1 l'_2 \rangle &\geq -1\\
-\langle l'_1 \rangle + \langle l'_2 \rangle - \langle l'_1 l'_2 \rangle &\geq -1\\
\langle l'_1 \rangle + \langle l'_2 \rangle + \langle l'_1 l'_2 \rangle &\geq -1\\
-\langle l'_1 \rangle - \langle l'_2 \rangle + \langle l'_1 l'_2 \rangle &\geq -1
